Add a new compilation pipeline example

fiat2/src/fiat2/PipelineEx.v
@@ -1,10 +1,13 @@
 Require Import fiat2.Language fiat2.Interpret fiat2.Value fiat2.TypeSystem fiat2.TypeSound fiat2.IndexInterface2
-fiat2.CollectionTransf fiat2.DictIndexImpl2 fiat2.SumAgg fiat2.BitmapIndex fiat2.TransfUtils fiat2.RelTransf fiat2.IndexTransf2 fiat2.TransfSound fiat2.Utils fiat2.Substitute.
+  fiat2.CollectionTransf fiat2.DictIndexImpl2 fiat2.SumAgg fiat2.BitmapIndex fiat2.TransfUtils fiat2.RelTransf fiat2.IndexTransf2 fiat2.TransfSound fiat2.Utils fiat2.Substitute.
 Require Import coqutil.Map.Interface coqutil.Map.SortedListString coqutil.Word.Interface coqutil.Datatypes.Result.
 Require Import List String ZArith.
 Import ListNotations.
 
-Section ConcreteExample.
+Require Import fiat2.Notations.
+Open Scope fiat2_scope.
+
+Section WithConcreteMaps.
   Context {width: Z} {word: word.word width} {word_ok: word.ok word}.
   Notation value := (value (width:=width)).
 
@@ -16,135 +19,233 @@ Section ConcreteExample.
   Instance clocals : map.map string value := SortedListString.map _.
   Instance clocals_ok : map.ok clocals := SortedListString.ok _.
 
-  Definition sum_agg_attr := "salary".
+  Section Example1.
+    Definition sum_agg_attr := "salary".
 
-  Notation sum_agg_wf := (SumAgg.idx_wf "hole" sum_agg_attr "x").
-  Instance csum_agg : IndexInterface2.index := (sum_agg "hole" sum_agg_attr "x").
-  Instance csum_agg_ok : IndexInterface2.ok csum_agg sum_agg_wf.
-  apply sum_agg_ok.
-  Qed.
+    Notation sum_agg_wf := (SumAgg.idx_wf "hole" sum_agg_attr "x").
+    Instance csum_agg : IndexInterface2.index := (sum_agg "hole" sum_agg_attr "x").
+    Instance csum_agg_ok : IndexInterface2.ok csum_agg sum_agg_wf.
+    apply sum_agg_ok.
+    Qed.
 
-  Definition dict_idx_attr := "department".
+    Definition dict_idx_attr := "department".
 
-  Notation dict_idx_wf := (DictIndexImpl2.idx_wf "hole" dict_idx_attr "tup" "acc" "x").
-  Instance cdict_idx : IndexInterface2.index := (dict_idx "hole" dict_idx_attr "tup" "acc" "x").
-  Instance cdict_idx_ok : IndexInterface2.ok cdict_idx dict_idx_wf.
-  apply dict_idx_ok. auto with transf_hints.
-  Qed.
+    Notation dict_idx_wf := (DictIndexImpl2.idx_wf "hole" dict_idx_attr "tup" "acc" "x").
+    Instance cdict_idx : IndexInterface2.index := (dict_idx "hole" dict_idx_attr "tup" "acc" "x").
+    Instance cdict_idx_ok : IndexInterface2.ok cdict_idx dict_idx_wf.
+    apply dict_idx_ok. auto with transf_hints.
+    Qed.
 
-  Notation pk_idx_wf := (BitmapIndex.pk_idx_wf "hole" "tup" "acc").
-  Instance cpk_idx : IndexInterface2.index := (pk_idx "hole" "tup" "acc").
-  Instance cpk_idx_ok : IndexInterface2.ok cpk_idx pk_idx_wf.
-  apply pk_idx_ok. auto with transf_hints.
-  Qed.
+    Notation pk_idx_wf := (BitmapIndex.pk_idx_wf "hole" "tup" "acc").
+    Instance cpk_idx : IndexInterface2.index := (pk_idx "hole" "tup" "acc").
+    Instance cpk_idx_ok : IndexInterface2.ok cpk_idx pk_idx_wf.
+    apply pk_idx_ok. auto with transf_hints.
+    Qed.
 
-  Definition bitmap_attr := "state".
-  Definition bitmap_str := "MA".
-  Notation bitmap_wf := (bitmap_wf bitmap_attr bitmap_str "hole" "tup").
-  Instance bitmap : IndexInterface2.index := (bitmap bitmap_attr bitmap_str "hole" "tup").
-  Instance bitmap_ok : IndexInterface2.ok bitmap bitmap_wf.
-  apply bitmap_ok.
-  Qed.
+    Definition bitmap_attr := "location".
+    Definition bitmap_str := "A".
+    Notation bitmap_wf := (bitmap_wf bitmap_attr bitmap_str "hole" "tup").
+    Instance bitmap : IndexInterface2.index := (bitmap bitmap_attr bitmap_str "hole" "tup").
+    Instance bitmap_ok : IndexInterface2.ok bitmap bitmap_wf.
+    apply bitmap_ok.
+    Qed.
 
-  Definition to_proj_transf := fold_command id to_proj_head.
-  Definition to_filter_transf := fold_command id to_filter_head.
-  Definition annotate_collection_transf := fold_command id annotate_collection.
-  Definition push_down_collection_transf := fold_command id push_down_collection.
-  Definition sum_agg_lookup_transf := fun tbl => fold_command_with_globals [tbl] (sum_to_agg_lookup_head sum_agg_attr "id_tag" "aux_tag" "sum_agg_tag" tbl).
-  Definition cons_to_add_transf := fun tbl => fold_command_with_globals [tbl] (cons_to_add_head).
-  Definition dict_lookup_transf := fun tbl => fold_command_with_globals [tbl] (eq_filter_to_lookup_head dict_idx_attr "id_tag" "aux_tag" "dict_idx_tag" "b" tbl).
-  Definition cons_to_insert_transf := fun tbl => fold_command_with_globals [tbl] (cons_to_insert_head dict_idx_attr "tup" "acc" "x" "y").
-  Definition use_dict_idx_transf := fun tbl => fold_command_with_globals [tbl] (use_idx_head dict_idx_attr "id_tag" "aux_tag" "dict_idx_tag" tbl).
-  Definition cons_to_pk_idx_update_transf := fun tbl => fold_command_with_globals [tbl] (cons_to_pk_idx_update_head "y").
-  Definition use_pk_idx_transf := fun tbl => fold_command_with_globals [tbl] (use_pk_idx_head "id_tag" "aux_tag" "pk_idx_tag" tbl).
-  Definition cons_to_bitmap_update_transf := fun tbl => fold_command_with_globals [tbl] cons_to_bitmap_update_head.
-  Definition use_bitmap_transf := fun tbl => fold_command_with_globals [tbl] (use_bitmap_head bitmap_attr bitmap_str "id_tag" "aux_tag" "bm_tag" tbl).
-  Definition filter_to_bitmap_lookup_transf :=
-    fun tbl => fold_command_with_globals [tbl]
-                 (filter_to_bitmap_lookup_head bitmap_attr bitmap_str "id_tag" "aux_tag" "pk_idx_tag" "bm_tag" "x" "b" "acc" tbl).
+    Definition to_proj_transf := fold_command id to_proj_head.
+    Definition to_filter_transf := fold_command id to_filter_head.
+    Definition annotate_collection_transf := fold_command id annotate_collection.
+    Definition push_down_collection_transf := fold_command id push_down_collection.
+    Definition sum_agg_lookup_transf := fun tbl => fold_command_with_globals [tbl] (sum_to_agg_lookup_head sum_agg_attr "id_tag" "aux_tag" "sum_agg_tag" tbl).
+    Definition cons_to_add_transf := fun tbl => fold_command_with_globals [tbl] (cons_to_add_head).
+    Definition dict_lookup_transf := fun tbl => fold_command_with_globals [tbl] (eq_filter_to_lookup_head dict_idx_attr "id_tag" "aux_tag" "dict_idx_tag" "b" tbl).
+    Definition cons_to_insert_transf := fun tbl => fold_command_with_globals [tbl] (cons_to_insert_head dict_idx_attr "tup" "acc" "x" "y").
+    Definition use_dict_idx_transf := fun tbl => fold_command_with_globals [tbl] (use_idx_head dict_idx_attr "id_tag" "aux_tag" "dict_idx_tag" tbl).
+    Definition cons_to_pk_idx_update_transf := fun tbl => fold_command_with_globals [tbl] (cons_to_pk_idx_update_head "y").
+    Definition use_pk_idx_transf := fun tbl => fold_command_with_globals [tbl] (use_pk_idx_head "id_tag" "aux_tag" "pk_idx_tag" tbl).
+    Definition cons_to_bitmap_update_transf := fun tbl => fold_command_with_globals [tbl] cons_to_bitmap_update_head.
+    Definition use_bitmap_transf := fun tbl => fold_command_with_globals [tbl] (use_bitmap_head bitmap_attr bitmap_str "id_tag" "aux_tag" "bm_tag" tbl).
+    Definition filter_to_bitmap_lookup_transf :=
+      fun tbl => fold_command_with_globals [tbl]
+                   (filter_to_bitmap_lookup_head bitmap_attr bitmap_str "id_tag" "aux_tag" "pk_idx_tag" "bm_tag" "x" "b" "acc" tbl).
 
-  Notation idxs := [("sum_agg_tag", csum_agg, sum_agg_wf);
-                    ("dict_idx_tag", cdict_idx, dict_idx_wf);
-                    ("pk_idx_tag", cpk_idx, pk_idx_wf);
-                    ("bm_tag", bitmap, bitmap_wf)].
-  Instance ccompo_idx : IndexInterface2.index := compo_idx idxs "hole" (word:=word).
-  Instance ccompo_idx_ok : IndexInterface2.ok ccompo_idx (compo_idx_wf idxs).
-  apply compo_idx_ok; repeat constructor; intros; auto with transf_hints.
-  all: cbn; rewrite <- eqb_eq; intuition idtac; discriminate.
-  Qed.
+    Notation idxs := [("sum_agg_tag", csum_agg, sum_agg_wf);
+                      ("dict_idx_tag", cdict_idx, dict_idx_wf);
+                      ("pk_idx_tag", cpk_idx, pk_idx_wf);
+                      ("bm_tag", bitmap, bitmap_wf)].
+    Instance ccompo_idx : IndexInterface2.index := compo_idx idxs "hole" (word:=word).
+    Instance ccompo_idx_ok : IndexInterface2.ok ccompo_idx (compo_idx_wf idxs).
+    apply compo_idx_ok; repeat constructor; intros; auto with transf_hints.
+    all: cbn; rewrite <- eqb_eq; intuition idtac; discriminate.
+    Qed.
 
-  Definition ex_transf (Gstore Genv : ctenv) :=
-    Basics.compose
-      (apply_idx_related_transfs (idx:=ccompo_idx) "id_tag" "aux_tag"
-         (fun tbl =>
-            (Basics.compose (filter_to_bitmap_lookup_transf tbl)
-               (Basics.compose (use_bitmap_transf tbl)
-                  (Basics.compose (repeat_transf (cons_to_bitmap_update_transf tbl) 10000)
-                        (Basics.compose (use_pk_idx_transf tbl)
-                           (Basics.compose (repeat_transf (cons_to_pk_idx_update_transf tbl) 10000)
-                                 (Basics.compose (dict_lookup_transf tbl)
-                                    (Basics.compose (use_dict_idx_transf tbl)
-                                       (Basics.compose (repeat_transf (cons_to_insert_transf tbl) 10000)
-                                             (Basics.compose (sum_agg_lookup_transf tbl)
-                                                (Basics.compose (repeat_transf (cons_to_add_transf tbl) 10000)
-                                                   (cons_to_add_transf tbl)))))))))))) Gstore Genv)
-      (Basics.compose push_down_collection_transf
-         (Basics.compose push_down_collection_transf
-            (Basics.compose annotate_collection_transf
-               (Basics.compose to_filter_transf to_proj_transf)))).
+    Definition ex_transf1 (Gstore Genv : ctenv) :=
+      Basics.compose
+        (apply_idx_related_transfs (idx:=ccompo_idx) "id_tag" "aux_tag"
+           (fun tbl =>
+              (Basics.compose (filter_to_bitmap_lookup_transf tbl)
+                 (Basics.compose (use_bitmap_transf tbl)
+                    (Basics.compose (repeat_transf (cons_to_bitmap_update_transf tbl) 10000)
+                       (Basics.compose (use_pk_idx_transf tbl)
+                          (Basics.compose (repeat_transf (cons_to_pk_idx_update_transf tbl) 10000)
+                             (Basics.compose (dict_lookup_transf tbl)
+                                (Basics.compose (use_dict_idx_transf tbl)
+                                   (Basics.compose (repeat_transf (cons_to_insert_transf tbl) 10000)
+                                      (Basics.compose (sum_agg_lookup_transf tbl)
+                                         (Basics.compose (repeat_transf (cons_to_add_transf tbl) 10000)
+                                            (cons_to_add_transf tbl)))))))))))) Gstore Genv)
+        (Basics.compose push_down_collection_transf
+           (Basics.compose push_down_collection_transf
+              (Basics.compose annotate_collection_transf
+                 (Basics.compose to_filter_transf to_proj_transf)))).
 
-  Lemma ex_transf_sound : transf_sound (locals:=clocals) ex_transf.
-  Proof.
-    repeat (repeat apply_transf_sound_lemmas; eauto 10 with transf_hints).
-  Qed.
+    Lemma ex_transf1_sound : transf_sound (locals:=clocals) ex_transf1.
+    Proof.
+      repeat (repeat apply_transf_sound_lemmas; eauto 10 with transf_hints).
+    Qed.
 
-  Require Import fiat2.Notations.
-  Open Scope fiat2_scope.
+    Definition row_ty := TRecord (record_sort [("name", TString); ("department", TString); ("feedback", TString); ("salary", TInt); ("location", TString)]).
+    (* Two Arbitrary well_typed rows *)
+    Definition row1 := EVar "row1".
+    Definition row2 := EVar "row2".
+    (* ??? change the names *)
 
-  Definition row_ty := TRecord (record_sort [("name", TString); ("department", TString); ("feedback", TString); ("salary", TInt); ("state", TString)]).
-  (* Two Arbitrary well_typed rows *)
-  Definition row1 := EVar "row1".
-  Definition row2 := EVar "row2".
-  (* ??? change the names *)
+    Definition build_responses1 := <{ set "responses" := row1 :: row2 :: mut "responses" }>.
+    Definition filter_responses dpt : expr := ESort LikeList <[ "row" <- mut "responses" ;
+                                                                check("row"["department"] == << EAtom (AString dpt) >>);
+                                                                ret "row" ]>.
+    (* ??? foreach from another table to update this table e.g. purchase of items*)
+    Definition filter_responses2 : expr := <[ "row" <- mut "responses" ;
+                                              check("row"["location"] == << EAtom (AString "A") >>);
+                                              ret "row" ]>.
+    Definition query1_1 := CForeach (filter_responses "CS") "r"
+                           <{ let "name" = "r"["name"] +++ << EAtom (AString ": ") >> in
+                              let "feedback" = "r"["feedback"] +++ << EAtom (AString "\n") >> in
+                              let "line" = "name" +++ "feedback" in
+                              set "all_feedback" := mut "all_feedback" +++ "line" }>.
+    Definition query1_2 := CAssign "sum" (EFold (<["row" <- mut "responses" ; ret "row"["salary"]]>) (EAtom (AInt 0)) "v" "acc" (EBinop OPlus (EVar "v") (EVar "acc"))).
+    Definition query1_3 := CForeach (filter_responses2) "r"
+                           <{ let "name" = "r"["name"] +++ << EAtom (AString ": ") >> in
+                              let "feedback" = "r"["feedback"] +++ << EAtom (AString "\n") >> in
+                              let "line" = "name" +++ "feedback" in
+                              set "all_feedback" := mut "all_feedback" +++ "line" }>.
+    Definition ex1' := CSeq build_responses1 (CSeq query1_1 (CSeq query1_2 query1_3)).
+    Definition ex1 := CLetMut (EAtom (ANil (Some (row_ty)))) "responses" ex1'.
 
-  Definition build_responses1 := <{ set "responses" := row1 :: row2 :: mut "responses" }>.
-  Definition filter_responses dpt : expr := ESort LikeList <[ "row" <- mut "responses" ;
-                                                       check("row"["department"] == << EAtom (AString dpt) >>);
-                                                              ret "row" ]>.
-  (* ??? foreach from another table to update this table e.g. purchase of items*)
-  Definition filter_responses2 : expr := <[ "row" <- mut "responses" ;
-                                            check("row"["state"] == << EAtom (AString "MA") >>);
-                                            ret "row" ]>.
-  Definition query1 := CForeach (filter_responses "EECS") "r"
-                      <{ let "name" = "r"["name"] +++ << EAtom (AString ": ") >> in
-                         let "feedback" = "r"["feedback"] +++ << EAtom (AString "\n") >> in
-                         let "line" = "name" +++ "feedback" in
-                         set "all_feedback" := mut "all_feedback" +++ "line" }>.
-  Definition query2 := CAssign "sum" (EFold (<["row" <- mut "responses" ; ret "row"["salary"]]>) (EAtom (AInt 0)) "v" "acc" (EBinop OPlus (EVar "v") (EVar "acc"))).
-  Definition query3 := CForeach (filter_responses2) "r"
-                      <{ let "name" = "r"["name"] +++ << EAtom (AString ": ") >> in
-                         let "feedback" = "r"["feedback"] +++ << EAtom (AString "\n") >> in
-                         let "line" = "name" +++ "feedback" in
-                         set "all_feedback" := mut "all_feedback" +++ "line" }>.
-  Definition ex1' := CSeq build_responses1 (CSeq query1 (CSeq query2 query3)).
-  Definition ex1 := CLetMut (EAtom (ANil (Some (row_ty)))) "responses" ex1'.
+    Definition init_Gstore1 : ctenv := map.put (map.put map.empty "all_feedback" TString) "sum" TInt.
+    Definition init_Genv1 : ctenv := map.put (map.put map.empty "row1" row_ty) "row2" row_ty.
 
-  Definition init_Gstore : ctenv := map.put (map.put map.empty "all_feedback" TString) "sum" TInt.
-  Definition init_Genv : ctenv := map.put (map.put map.empty "row1" row_ty) "row2" row_ty.
+    (* Compute typecheck init_Gstore1 init_Genv1 ex1. *)
 
-  Compute typecheck init_Gstore init_Genv ex1.
+    Definition ex1_transformed := ex_transf1 init_Gstore1 init_Genv1 ex1.
+    (* Compute ex1_transformed. *)
 
-  Unset Printing Notations.
-  Definition ex1_transformed := ex_transf init_Gstore init_Genv ex1.
-  Compute ex1_transformed.
+    Theorem ex1_transformed_sem : forall (store env : clocals),
+        locals_wf init_Gstore1 store ->
+        locals_wf init_Genv1 env ->
+        interp_command store env ex1_transformed = interp_command store env ex1.
+    Proof.
+      apply transf_sound__preserve_sem; auto using ex_transf1_sound with transf_hints.
+    Qed.
+  End Example1.
 
-  Theorem ex1_transformed_sem : forall (store env : clocals),
-      locals_wf init_Gstore store ->
-      locals_wf init_Genv env ->
-      interp_command store env ex1_transformed = interp_command store env ex1.
-  Proof.
-    intros. apply transf_sound__preserve_sem; auto using ex_transf_sound with transf_hints.
-  Qed.
-End ConcreteExample.
+  Section Example2.
+    Definition sum_agg_attr2 := "price".
+
+    Notation sum_agg_wf2 := (SumAgg.idx_wf "hole" sum_agg_attr2 "x").
+    Instance csum_agg2 : IndexInterface2.index := (sum_agg "hole" sum_agg_attr2 "x").
+    Instance csum_agg_ok2 : IndexInterface2.ok csum_agg2 sum_agg_wf2.
+    apply sum_agg_ok.
+    Qed.
+
+    Definition dict_idx_attr2 := "color".
+
+    Notation dict_idx_wf2 := (DictIndexImpl2.idx_wf "hole" dict_idx_attr2 "tup" "acc" "x").
+    Instance cdict_idx2 : IndexInterface2.index := (dict_idx "hole" dict_idx_attr2 "tup" "acc" "x").
+    Instance cdict_idx_ok2 : IndexInterface2.ok cdict_idx2 dict_idx_wf2.
+    apply dict_idx_ok. auto with transf_hints.
+    Qed.
+
+    Definition sum_agg_lookup_transf2 := fun tbl => fold_command_with_globals [tbl] (sum_to_agg_lookup_head sum_agg_attr2 "id_tag" "aux_tag" "sum_agg_tag" tbl).
+    Definition cons_to_add_transf2 := fun tbl => fold_command_with_globals [tbl] (cons_to_add_head).
+    Definition dict_lookup_transf2 := fun tbl => fold_command_with_globals [tbl] (eq_filter_to_lookup_head dict_idx_attr2 "id_tag" "aux_tag" "dict_idx_tag" "b" tbl).
+    Definition cons_to_insert_transf2 := fun tbl => fold_command_with_globals [tbl] (cons_to_insert_head dict_idx_attr2 "tup" "acc" "x" "y").
+    Definition use_dict_idx_transf2 := fun tbl => fold_command_with_globals [tbl] (use_idx_head dict_idx_attr2 "id_tag" "aux_tag" "dict_idx_tag" tbl).
+
+    Notation idxs2 := [("sum_agg_tag", csum_agg2, sum_agg_wf2);
+                       ("dict_idx_tag", cdict_idx2, dict_idx_wf2)].
+    Instance ccompo_idx2 : IndexInterface2.index := compo_idx idxs2 "hole" (word:=word).
+    Instance ccompo_idx_ok2 : IndexInterface2.ok ccompo_idx2 (compo_idx_wf idxs2).
+    apply compo_idx_ok; repeat constructor; intros; auto with transf_hints.
+    all: cbn; rewrite <- eqb_eq; intuition idtac; discriminate.
+    Qed.
+
+    Definition ex_transf2 (Gstore Genv : ctenv) :=
+      Basics.compose
+        (apply_idx_related_transfs (idx:=ccompo_idx2) "id_tag" "aux_tag"
+           (fun tbl =>
+              (Basics.compose (dict_lookup_transf2 tbl)
+                 (Basics.compose (use_dict_idx_transf2 tbl)
+                    (Basics.compose (repeat_transf (cons_to_insert_transf2 tbl) 10000)
+                       (Basics.compose (sum_agg_lookup_transf2 tbl)
+                          (Basics.compose (repeat_transf (cons_to_add_transf2 tbl) 10000)
+                             (cons_to_add_transf2 tbl))))))) Gstore Genv)
+        (Basics.compose push_down_collection_transf
+           (Basics.compose push_down_collection_transf
+              (Basics.compose annotate_collection_transf
+                 (Basics.compose to_filter_transf to_proj_transf)))).
+
+    Lemma ex_transf2_sound : transf_sound (locals:=clocals) ex_transf2.
+    Proof.
+      repeat (repeat apply_transf_sound_lemmas; eauto 10 with transf_hints).
+    Qed.
+
+    Definition outfits_row_ty := TRecord (record_sort [("outfit_name", TString); ("shirt_name", TString); ("shirt_color", TString); ("shirt_price", TInt); ("pants_name", TString); ("pants_color", TString); ("pants_price", TInt)]).
+
+    Definition shirts_row_ty := TRecord (record_sort [("name", TString); ("color", TString); ("price", TInt)]).
+
+    Definition populate_shirts_from_outfits : command :=
+      CForeach (EFlatmap LikeList (ELoc "outfits") "row"
+                  (EBinop OCons
+                     (ERecord [("name", EAccess (EVar "row") "shirt_name"); ("color", EAccess (EVar "row") "shirt_color"); ("price", EAccess (EVar "row") "shirt_price")])
+                     (EAtom (ANil (Some shirts_row_ty)))))
+        "row" (CAssign "shirts" (EBinop OCons (EVar "row") (ELoc "shirts"))).
+
+    Definition filter_shirts color : expr :=
+      ESort LikeList <[ "row" <- mut "shirts" ;
+                        check("row"["color"] == << EAtom (AString color) >>);
+                        ret "row" ]>.
+
+    Definition query2_1 :=
+      CLetMut (EAtom (AString ""))  "all_shirt_info"
+        (CForeach (filter_shirts "white") "r"
+         <{ let "n" = "r"["name"] +++ << EAtom (AString ": ") >> in
+            let "p" = << EUnop OIntToString (EAccess (EVar "r") "price") >> +++ << EAtom (AString "\n") >> in
+            let "line" = "n" +++ "p" in
+            set "all_shirt_info" := mut "all_shirt_info" +++ "line" }>).
+
+    Definition query2_2 :=
+      CLetMut (EFold (<["row" <- mut "shirts" ; ret "row"["price"]]>) (EAtom (AInt 0)) "v" "acc" (EBinop OPlus (EVar "v") (EVar "acc"))) "total_shirt_price" CSkip.
+
+    Definition ex2 := CLetMut (EAtom (ANil (Some (shirts_row_ty)))) "shirts"
+                        (CSeq populate_shirts_from_outfits
+                           (CSeq query2_1 query2_2)).
+
+    Definition init_Gstore2 : ctenv := map.put map.empty "outfits" (TList outfits_row_ty).
+    Definition init_Genv2 : ctenv := map.empty.
+
+    (* Compute typecheck init_Gstore2 init_Genv2 ex2. *)
+
+    Definition ex2_transformed := ex_transf2 init_Gstore2 init_Genv2 ex2.
+    (* Compute ex2_transformed. *)
+
+    Theorem ex2_transformed_sem : forall (store env : clocals),
+        locals_wf init_Gstore2 store ->
+        locals_wf init_Genv2 env ->
+        interp_command store env ex2_transformed = interp_command store env ex2.
+    Proof.
+      apply transf_sound__preserve_sem; auto using ex_transf2_sound with transf_hints.
+    Qed.
+  End Example2.
+End WithConcreteMaps.
 
 Print Assumptions ex1_transformed.
+Print Assumptions ex2_transformed.
